SAW/spec/EC/Coq/EC_fiat_P384_gen.v
@@ -1,0 +1,1229 @@
+
+Set Implicit Arguments.
+
+From Coq Require Import Lists.List.
+From Coq Require Import String.
+From Coq Require Import Vectors.Vector.
+From Coq Require Import Vectors.VectorSpec.
+From Coq Require Import Lia.
+
+
+From CryptolToCoq Require Import SAWCoreScaffolding.
+From CryptolToCoq Require Import SAWCoreVectorsAsCoqVectors.
+Import ListNotations.
+
+From CryptolToCoq Require Import CryptolPrimitivesForSAWCore.
+Import CryptolPrimitivesForSAWCore.
+From CryptolToCoq Require Import CryptolPrimitivesForSAWCoreExtra.
+From CryptolToCoq Require Import SAWCorePrelude.
+Import SAWCorePrelude.
+
+From CryptolToCoq Require Import SAWCoreBitvectors.
+
+From Top Require Import EC_fiat_P384_7.
+
+
+Definition append_comm (m n : Nat) (a : Type) (Inh_a : Inhabited a) 
+  (x : Vec m a) (y : Vec n a) :=
+gen (addNat n m) a
+  (fun i : Nat =>
+   if ltNat i m then sawAt m a x i else sawAt n a y (subNat i m)).
+
+
+Local Arguments cons [_] h [_] t.
+Local Arguments append [m] [n] [a]%type_scope {Inh_a} x y.
+Local Arguments append_comm [m] [n] [a]%type_scope {Inh_a} x y.
+Local Arguments bvOr [n] _ _.
+Local Arguments bvAnd [n] _ _.
+Local Arguments reverse [n] [a]%type_scope {Inh_a} _.
+Local Arguments bvSub [n] _ _.
+Local Arguments SAWCorePrelude.map [a]%type_scope {Inh_a} [b]%type_scope f%function_scope _ _.
+
+
+
+
+Definition fiat_mul_scalar_rwnaf_odd_loop_body_gen (wsize : nat)(s : bitvector 384) :=
+(drop Bool 368 16
+   (bvSub
+      (bvURem 384 s
+         (bvMul 384 (bvNat 384 2)
+            (shiftL 384 bool false (bvNat 384 1) wsize)))
+      (shiftL 384 bool false (bvNat 384 1) wsize)),
+shiftR 384 bool false
+  (bvSub s
+     (bvSub
+        (bvURem 384 s
+           (bvMul 384 (bvNat 384 2)
+              (shiftL 384 bool false (bvNat 384 1) wsize)))
+        (shiftL 384 bool false (bvNat 384 1) wsize))) wsize).
+
+Ltac ecSimpl_one :=
+  match goal with
+    | [ |- context[ecNumber (TCNum ?a) ?t (PLiteralSeqBool (TCNum ?s))]] =>
+        replace (ecNumber (TCNum a) t (PLiteralSeqBool (TCNum s))) with (bvNat s a); [idtac | reflexivity] 
+    | [ |- context[ecNumber (TCNum ?a) ?t PLiteralInteger]] =>
+        replace (ecNumber (TCNum a) t PLiteralInteger) with (Z.of_nat a); [idtac | reflexivity] 
+    | [|- context[ecCat ?s1 ?s2 ?t ?a ?b]] =>
+        replace (ecCat s1 s2 t a b) with (append a b); [idtac | reflexivity]
+    | [|- context[map ?s ?t1 ?t2 ?f ?ls]] =>
+        replace (map s t1 t2 f ls) with (SAWCorePrelude.map f _ ls); [idtac | reflexivity]
+    | [ |- context[ecPlus Integer ?r (Z.of_nat ?a) (Z.of_nat ?b)]] =>
+        replace (ecPlus Integer r (Z.of_nat a) (Z.of_nat b)) with (ecNumber (a + b) Integer PLiteralInteger); [idtac | reflexivity]
+    | [ |- context[ecMinus ?t (PRingSeqBool ?s) ?a ?b]] => 
+        replace (ecMinus t (PRingSeqBool s) a b) with (bvSub a b); [idtac | reflexivity]
+    | [ |- context[ecPlus ?t (PRingSeqBool ?s) ?a ?b]] => 
+        replace (ecPlus t (PRingSeqBool s) a b) with (bvAdd a b); [idtac | reflexivity]
+    | [ |- context[ecAnd ?t (PLogicSeqBool ?s) ?a ?b]] => 
+        replace (ecAnd t (PLogicSeqBool s) a b) with (bvAnd a b); [idtac | reflexivity]
+    | [ |- context[ecMul ?t (PRingSeqBool ?s) ?a ?b]] => 
+        replace (ecMul t (PRingSeqBool s) a b) with (bvMul _ a b); [idtac | reflexivity]
+    | [ |- context[ecMod ?t (PIntegralSeqBool ?s) ?a ?b]] => 
+        replace (ecMod t (PIntegralSeqBool s) a b) with (bvURem _ a b); [idtac | reflexivity]
+    | [ |- context[ecDrop (TCNum ?s1) (TCNum ?s2) ?t ?a]] => 
+        replace (ecDrop (TCNum s1) (TCNum s2) t a) with (drop _ s1 s2 a); [idtac | reflexivity]
+    | [ |- context[ecShiftL ?s ?t Bool ?r PZeroBit ?a (Z.of_nat ?b)]] => 
+        replace (ecShiftL s t Bool r PZeroBit a (Z.of_nat b)) with (shiftL _ _ false a b); [idtac | reflexivity]
+    | [ |- context[ecShiftR ?s1 ?t Bool ?r PZeroBit ?a (bvNat ?s2 ?b)]] => 
+        replace (ecShiftR s1 t Bool r PZeroBit a (bvNat s2 b)) with (shiftR _ _ false a b); [idtac | reflexivity]
+    | [ |- context[ecShiftR ?s ?t Bool ?r PZeroBit ?a (Z.of_nat ?b)]] => 
+        replace (ecShiftR s t Bool r PZeroBit a (Z.of_nat b)) with (shiftR _ _ false a b); [idtac | reflexivity]
+  end.
+
+Ltac removeCoerce :=
+  match goal with
+  | [ |- context[coerce ?t1 ?t2 ?p ?a]] => 
+    replace (coerce t1 t2 p a) with a; [idtac | reflexivity]
+  end.
+
+Theorem fiat_mul_scalar_rwnaf_odd_loop_body_gen_equiv : forall s,
+  fiat_mul_scalar_rwnaf_odd_loop_body_gen 7 s = fiat_mul_scalar_rwnaf_odd_loop_body s.
+
+  intros.
+  unfold fiat_mul_scalar_rwnaf_odd_loop_body, fiat_mul_scalar_rwnaf_odd_loop_body.
+  repeat ecSimpl_one.
+  removeCoerce.
+  reflexivity.
+
+Qed.
+
+
+Theorem ecScanl_vec_ext : forall t1 t2 (f1 f2 : t1 -> t2 -> t1) n (ls : Vec n t2) x,
+  (forall x y, f1 x y = f2 x y) ->
+  (ecScanl n t1 t2 f1 x ls) = (ecScanl n t1 t2 f2 x ls).
+
+  induction ls; intros.
+  reflexivity.
+
+  simpl.
+  rewrite H.
+  f_equal.
+  eapply IHls; eauto.
+
+Qed.
+
+Fixpoint toN_excl_int n :=
+  match n with 
+  | 0 => List.nil
+  | S n' => (toN_excl_int n') ++ (Z.of_nat n') :: List.nil
+  end.
+
+Definition toN_int n :=
+  (toN_excl_int n) ++ ((Z.of_nat n) :: List.nil).
+
+Theorem ecFromTo_0_n_equiv : forall n,
+  to_list (ecFromTo 0 (TCNum n) Integer PLiteralInteger) = 
+  (toN_int n).
+
+  intros.
+  unfold ecFromTo, toN_int.
+  simpl.
+
+Admitted.
+
+Fixpoint toN_excl_bv s n :=
+  match n with 
+  | 0 => List.nil
+  | S n' => (toN_excl_bv s n') ++ (bvNat s n') :: List.nil
+  end.
+
+Definition toN_bv s n :=
+  (toN_excl_bv s n) ++ ((bvNat s n) :: List.nil).
+
+Theorem ecFromTo_0_n_bv_excl_equiv : forall (s : nat) n,
+  to_list (ecFromTo 0 (TCNum n) (CryptolPrimitivesForSAWCore.seq (TCNum s) Bool)
+           (PLiteralSeqBool (TCNum s))) = 
+  (toN_excl_bv s (S n)).
+
+Admitted.
+
+Theorem ecFromTo_0_n_bv_equiv : forall (s : nat) n,
+  to_list (ecFromTo 0 (TCNum n) (CryptolPrimitivesForSAWCore.seq (TCNum s) Bool)
+           (PLiteralSeqBool (TCNum s))) = 
+  (toN_bv s n).
+
+Admitted.
+
+
+Theorem ecFromTo_m_n_equiv : forall m n,
+  to_list (ecFromTo (TCNum m) (TCNum n) Integer PLiteralInteger) = 
+  (List.map (Z.add (Z.of_nat m)) (toN_int (n-m))).
+
+Admitted.
+
+Theorem toList_ecDrop_equiv : forall A (inh : Inhabited A) n m (v : Vec (addNat n m) A),
+  to_list (ecDrop n m _ v) = skipn n (to_list v).
+
+Admitted.
+
+Theorem toList_append_equiv : forall A (inh : Inhabited A) n m (v1 : Vec n A)(v2 : Vec m A),
+  to_list (append v1 v2) = 
+  List.app (to_list v1) (to_list v2).
+
+Admitted.
+
+Theorem toList_map_equiv : forall A (inh : Inhabited A) B n (v : Vec n A) (f : A -> B),
+  to_list (SAWCorePrelude.map f _ v) = List.map f (to_list v).
+
+Admitted.
+
+Theorem toList_cons : forall A n (v : Vec n A) a,
+  to_list (cons a v) = List.cons a (to_list v).
+
+  intros.
+  reflexivity.
+
+Qed.
+
+Fixpoint scanl (A B : Type)(f : A -> B -> A)(ls : list B)(a : A) :=
+  match ls with 
+  | List.nil => a :: List.nil 
+  | b :: ls' => a :: scanl f ls' (f a b)
+  end.
+
+Theorem toList_scanl_equiv : forall (A B : Type)(f : A -> B -> A) n (v : Vec n B)(a : A),
+  to_list (ecScanl (TCNum n) A B f a v) = scanl f (to_list v) a.
+
+  induction v; intros.
+  simpl. reflexivity.
+
+  simpl.
+  rewrite toList_cons.
+  f_equal.
+  eapply IHv.
+
+Qed.
+
+Theorem ecAtBack_0_equiv : forall n A (inh : Inhabited A)(def : A) r (v : seq (TCNum n) A),
+  (@ecAtBack (TCNum n) A inh _ r v 0) = List.hd def (List.rev (to_list v)).
+    
+  intros.
+  unfold ecAtBack.
+
+Abort.
+
+Fixpoint scanl_fix (A C : Type)(f : A -> A)(f1 f2 : A -> C) n a := 
+  match n with
+  | 0 => List.nil
+  | 1 => (f1 a) :: (f2 a) :: List.nil
+  | S n' => (f1 a) :: (scanl_fix f f1 f2 n' (f a))
+  end.
+
+From Top Require Import GroupMulWNAF.
+Require Import ZArith.BinInt.
+Require Import BinNat.
+Require Import BinPos.
+Require Import Pnat.
+Require Import Nat.
+Require Import List.
+Require Import Arith.
+
+Definition fiat_mul_scalar_rwnaf_odd_gen wsize numWindows s :=
+  List.map (fun x : bitvector 16 * bitvector 384 => fst x)
+  (scanl
+     (fun (__p2 : bitvector 16 * bitvector 384) (_ : Integer) =>
+      fiat_mul_scalar_rwnaf_odd_loop_body_gen wsize (snd __p2)) (toN_int numWindows)
+     (fiat_mul_scalar_rwnaf_odd_loop_body_gen wsize s)) ++
+[drop Bool 368%nat 16%nat
+   (snd
+      (hd (inhabitant (Inhabited_prod (bitvector 16) (bitvector 384)))
+         (rev
+            (scanl
+               (fun (__p2 : bitvector 16 * bitvector 384) (_ : Integer) =>
+                fiat_mul_scalar_rwnaf_odd_loop_body_gen wsize (snd __p2)) 
+               (toN_int numWindows) (fiat_mul_scalar_rwnaf_odd_loop_body_gen wsize s)))))].
+
+
+Local Open Scope Z_scope.
+
+Definition recode_rwnaf_odd_scanl_fix_body wsize n :=
+      let k_i := (n mod (Z.double (twoToWsize wsize))) - (twoToWsize wsize) in
+      let n' := (n - k_i) / (twoToWsize wsize) in
+      (k_i, n').
+
+Theorem recode_rwnaf_odd_scanl_equiv : forall wsize nw (n : Z),
+  recode_rwnaf_odd wsize (S nw) n = 
+  scanl_fix 
+    (fun p => recode_rwnaf_odd_scanl_fix_body wsize (snd p))
+    (fun p => fst p)
+    (fun p => snd p)
+    (S nw) (recode_rwnaf_odd_scanl_fix_body wsize n).
+
+  induction nw; intros; simpl in *.
+  reflexivity.
+  rewrite IHnw.
+  reflexivity.
+Qed.
+
+
+Theorem hd_app_eq : forall (A : Type)(defA: A)(ls1 ls2 : list A),
+  length ls1 <> O ->
+  hd defA (ls1 ++ ls2) = hd defA ls1.
+
+  intros.
+  destruct ls1; simpl in *.
+  intuition.
+  trivial.
+Qed.
+
+Theorem scanl_length : forall (A B : Type)(ls : list A)(f : B -> A -> B)(b : B),
+  Datatypes.length (scanl f ls b) <> O.
+
+  intros.
+  destruct ls; simpl; intuition.
+
+Qed.
+
+
+Theorem scanl_fix_equiv : forall (A B C: Type) (defA : A) (f : A -> A) (ls : list B) (n : nat) (f1 f2 : A -> C) a,
+  List.length ls = n ->  
+  (List.map f1 (scanl (fun x y => f x) ls a)) ++ (f2 (List.hd defA (List.rev (scanl (fun x y => f x) ls a))))::List.nil = 
+  scanl_fix f f1 f2 (S n) a.
+
+  induction ls; destruct n; intros; simpl in *.
+  reflexivity.
+  discriminate.
+  discriminate.
+  
+  f_equal.
+
+  rewrite hd_app_eq.
+  eapply IHls.
+  lia.
+
+  rewrite rev_length.
+  eapply scanl_length.
+Qed.
+
+
+Theorem ecCat_equiv : forall s1 s2 t (inh : Inhabited t)(a : Vec s1 t) (b : Vec s2 t),
+  (ecCat (TCNum s1) (TCNum s2) t a b) = (append a b).
+
+  intros.
+  reflexivity.
+Qed.
+
+
+Theorem to_list_ecCAt_equiv : forall (s1 s2 : nat) t (inh : Inhabited t)(a : Vec s1 t) (b : Vec s2 t),
+  (to_list (ecCat (TCNum s1) (TCNum s2) t a b)) = (List.app (to_list a) (to_list b)).
+
+  intros.
+  rewrite ecCat_equiv.
+  apply toList_append_equiv.
+
+Qed.
+
+Theorem sawAt_nth_equiv : forall (A : Type)(inh : Inhabited A)(n1 : nat)(ls : Vec n1 A)(n2 : nat),
+   (n2 < n1)%nat ->
+   (sawAt _ _ ls n2) = (nth n2 (to_list ls) (inhabitant inh)).
+
+  induction ls; intros; simpl in *.
+  lia.
+
+  destruct n2; simpl in *.
+  trivial.
+
+  unfold sawAt in *. simpl.
+  rewrite IHls.
+  reflexivity.
+  lia.
+Qed.
+
+Theorem toList_reverse_equiv : forall (A : Type)(inh : Inhabited A) n (ls : Vec n A),
+  to_list (reverse ls) = rev (to_list ls).
+
+
+  induction ls; intros; simpl in *.
+  trivial.
+Admitted.
+
+Theorem nth_0_hd_equiv : forall (A : Type)(defA : A)(ls : list A),
+  nth 0 ls defA = hd defA ls.
+
+  destruct ls; trivial.
+
+Qed.
+
+Theorem scanl_ext : forall (A B : Type)(f1 f2 : A -> B -> A) ls a,
+    (forall a b, f1 a b = f2 a b) ->
+    (scanl f1 ls a) = (scanl f2 ls a).
+
+  induction ls; intuition idtac; simpl in *.
+  f_equal.
+  rewrite H.
+  eapply IHls.
+  eauto.
+
+Qed.
+
+Require Import Coq.ZArith.Zdigits.
+
+(*
+Theorem recode_rwnaf_odd_scanl_fix_body_equiv : forall wsize (s : bitvector 384),
+  fiat_mul_scalar_rwnaf_odd_loop_body_gen wsize s
+  = recode_rwnaf_odd_scanl_fix_body wsize (binary_value _ s).
+*)
+
+(* Take a gen function an simplify to it. Then prove that equivalent to the model *)
+Theorem fiat_mul_scalar_rwnaf_odd_gen_equiv : forall s,
+  to_list (fiat_mul_scalar_rwnaf_odd s) = (fiat_mul_scalar_rwnaf_odd_gen 7 52 s).
+
+  intros.
+  unfold fiat_mul_scalar_rwnaf_odd.
+  repeat removeCoerce.
+
+  Local Opaque append of_list ecFromTo.
+  simpl.
+
+  match goal with
+  | [|- context[to_list (append ?v1 ?v2 )]] =>
+    replace (to_list (append v1 v2 )) with (List.app (to_list v1) (to_list v2)); [idtac | symmetry; apply toList_append_equiv]
+  end.
+
+  rewrite toList_map_equiv.
+  match goal with
+  | [|- context[to_list (SAWCoreVectorsAsCoqVectors.scanl ?t1 ?t2 ?n ?f ?a ?v)]] =>
+    replace (to_list (SAWCoreVectorsAsCoqVectors.scanl t1 t2 n f a v)) with (scanl f (to_list v) a); [idtac | symmetry; apply toList_scanl_equiv]
+  end.
+
+  rewrite to_list_of_list_opp.
+  rewrite ecFromTo_0_n_equiv.
+  rewrite sawAt_nth_equiv.
+  rewrite toList_reverse_equiv.
+  rewrite nth_0_hd_equiv.
+  match goal with
+  | [|- context[to_list (SAWCoreVectorsAsCoqVectors.scanl ?t1 ?t2 ?n ?f ?a ?v)]] =>
+    replace (to_list (SAWCoreVectorsAsCoqVectors.scanl t1 t2 n f a v)) with (scanl f (to_list v) a); [idtac | symmetry; apply toList_scanl_equiv]
+  end.
+
+  rewrite <- fiat_mul_scalar_rwnaf_odd_loop_body_gen_equiv.
+  rewrite (scanl_ext _ (fun (__p2 : bitvector 16 * bitvector 384) (_ : Integer) =>
+      fiat_mul_scalar_rwnaf_odd_loop_body_gen 7 (snd __p2))).
+
+  rewrite ecFromTo_0_n_equiv.
+  trivial.
+
+  intros.
+  symmetry.
+  apply fiat_mul_scalar_rwnaf_odd_loop_body_gen_equiv.
+
+  lia.
+
+Qed.
+
+Theorem to_list_cons : forall (A : Type)(n : Nat)(ls : Vec n A) x,
+  to_list (VectorDef.cons x ls) = List.cons x (to_list ls).
+Admitted.
+
+Definition fiat_mul_scalar_rwnaf_gen wsize nw s := 
+  fiat_mul_scalar_rwnaf_odd_gen wsize nw
+    (bvOr s (intToBv 384%nat 1)).
+
+Theorem fiat_mul_scalar_rwnaf_equiv : forall s,
+  to_list (fiat_mul_scalar_rwnaf s) = fiat_mul_scalar_rwnaf_gen 7 52 s.
+
+  intros.
+  unfold fiat_mul_scalar_rwnaf.
+  rewrite fiat_mul_scalar_rwnaf_odd_gen_equiv.
+  Local Opaque fiat_mul_scalar_rwnaf_odd_gen.
+  simpl.
+  reflexivity.
+
+Qed.
+
+Theorem sawAt_3_equiv : forall A (inh : Inhabited A) (v : Vector.t A 3),
+  Vector.cons (sawAt 3%nat A v 0%nat)
+    (Vector.cons (sawAt 3%nat A v 1%nat)
+      (Vector.cons (sawAt 3%nat A v 2%nat) (Vector.nil A)))
+  = v.
+Admitted.
+
+Theorem sawAt_3_equiv_gen : forall A (inh : Inhabited A) (v1 v2 : Vector.t A 3),
+  v1 = v2 ->
+  Vector.cons (sawAt 3%nat A v1 0%nat)
+    (Vector.cons (sawAt 3%nat A v1 1%nat)
+      (Vector.cons (sawAt 3%nat A v1 2%nat) (Vector.nil A)))
+  = v2.
+  
+  intros.
+  subst.
+  apply sawAt_3_equiv.
+
+Qed.
+
+Theorem ecFoldl_foldl_equiv : forall (A B : Type)(inhB : Inhabited B)(f : A -> B -> A) n ls a,
+    ecFoldl (TCNum n) _ _ f a ls = fold_left f (to_list ls) a.
+
+Admitted.
+
+Theorem toList_ecReverse_equiv : forall (A : Type)(inh : Inhabited A) n (ls : Vec n A),
+  to_list (ecReverse (TCNum n) _ ls) = rev (to_list ls).
+    
+  intros.
+  simpl.
+  apply toList_reverse_equiv.
+Qed.
+
+Theorem toList_zip_equiv : forall (A B : Type)(inha : Inhabited A)(inhb: Inhabited B) n (lsa: Vec n A) (lsb : Vec n B),
+  to_list (zip (TCNum n) _ _ lsa lsb) = List.combine (to_list lsa) (to_list lsb).
+
+Admitted.
+
+Theorem ecAt_equiv : forall A s (ls : Vec s A) (n : Z) def,
+    (Z.to_nat n < s)%nat ->
+    ecAt (TCNum s) A _ PIntegralInteger ls n = nth (Z.to_nat n) (to_list ls) def.
+
+Admitted.
+
+Definition fiat_select_point_ct_gen x t :=
+  fold_left
+  (fun acc p =>
+   fiat_select_point_loop_body x acc (fst p) (snd p))
+  (combine (toN_excl_bv 64%nat (length t)) t) (of_list [zero_felem; zero_felem; zero_felem]).
+
+Theorem to_list_length : forall (A : Type)(n : nat)(x : Vector.t A n),
+  (List.length (to_list x)) = n.
+
+  induction x; intros. 
+  simpl in *; trivial.
+  rewrite to_list_cons.
+  simpl.
+  rewrite IHx.
+  trivial.
+
+Qed.
+
+
+Theorem fiat_select_point_ct_gen_equiv : forall x t,
+  fiat_select_point_ct x t = fiat_select_point_ct_gen x (to_list t).
+
+  intros.
+  unfold fiat_select_point_ct, fiat_select_point_ct_gen.
+  removeCoerce.
+  rewrite ecFoldl_foldl_equiv.
+  rewrite toList_zip_equiv. 
+
+  replace ((to_list
+        (ecFromTo 0%nat 63%nat (CryptolPrimitivesForSAWCore.seq 64%nat Bool)
+           (PLiteralSeqBool 64%nat))))
+  with (toN_excl_bv 64%nat (length (to_list t))).
+  reflexivity.
+  rewrite to_list_length.
+  symmetry.
+  apply (@ecFromTo_0_n_bv_excl_equiv 64%nat 63%nat).
+Qed.
+
+Theorem fold_left_ext : forall (A B : Type)(f1 f2 : A -> B -> A) ls a,
+    (forall a b, f1 a b = f2 a b) ->
+    fold_left f1 ls a = fold_left f2 ls a.
+
+  induction ls; intuition idtac; simpl in *.
+  rewrite H.
+  apply IHls.
+  intuition idtac.  
+Qed.
+
+Theorem toList_drop_equiv : forall A (inh : Inhabited A) n1 n2 ls,
+  to_list (drop A n1 n2 ls) = skipn n1 (to_list ls).
+
+Admitted.
+
+Section PointMul.
+
+  Definition felem := Vector.t (bitvector 64) 6.
+  Definition prodPoint := (felem * felem * felem)%type.
+  Definition point := Vector.t felem 3.
+  Variable field_square : felem -> felem.
+  Variable field_mul field_sub field_add : felem -> felem -> felem.
+  Variable field_opp : felem -> felem.
+
+  Definition fiat_point_opp (p : point) : point :=
+    Vector.cons (sawAt _ _ p 0%nat) 
+      (Vector.cons (field_opp (sawAt _ _ p 1%nat) ) 
+        (Vector.cons (sawAt _ _ p 2%nat)  (Vector.nil felem))).
+
+  Definition fiat_point_mul := fiat_point_mul field_square field_mul field_sub field_add field_opp.
+ 
+  Definition conditional_subtract_if_even_ct := 
+    conditional_subtract_if_even_ct field_square field_mul field_sub field_add field_opp.
+
+  Definition fiat_point_add := 
+    fiat_point_add field_square field_mul field_sub field_add.
+
+  Theorem conditional_subtract_if_even_ct_equiv : forall (p1 : point) n (p2 : point),
+    conditional_subtract_if_even_ct p1 n p2 = 
+    if (even (bvToNat _ n)) then (fiat_point_add false p1 (fiat_point_opp p2)) else p1.
+
+    intros.
+    unfold conditional_subtract_if_even_ct, EC_fiat_P384_7.conditional_subtract_if_even_ct.
+    unfold fiat_field_cmovznz.
+    match goal with
+    | [|- context[of_list [if ?a then _ else _; _; _]]] =>
+      case_eq a; intros
+    end.
+    unfold ecEq, ecAnd, ecZero, byte_to_limb in H. simpl in H.
+    case_eq (even (bvToNat 384%nat n)); intros.
+    (* both even *)
+    simpl.
+    Local Transparent of_list.
+    unfold of_list.
+    apply sawAt_3_equiv.
+
+    (* contradiction *)
+    admit.
+
+    case_eq (even (bvToNat 384%nat n)); intros.
+    (* contradiction *)
+    admit.
+
+    (* both odd. *)
+    unfold of_list. 
+    apply sawAt_3_equiv.
+
+  Admitted.
+
+  Definition fiat_pre_comp_table := fiat_pre_comp_table field_square field_mul field_sub field_add .
+
+  Definition fiat_pre_comp_table_gen pred_tsize p :=
+    scanl
+  (fun
+     (z : CryptolPrimitivesForSAWCore.seq 3%nat
+            (CryptolPrimitivesForSAWCore.seq 6%nat
+               (CryptolPrimitivesForSAWCore.seq 64%nat Bool))) 
+     (_ : Integer) =>
+   EC_fiat_P384_7.fiat_point_add field_square field_mul field_sub field_add
+     (ecNumber 0%nat Bool PLiteralBit)
+     (fiat_point_double field_square field_mul field_sub field_add p) z)
+  (map (BinIntDef.Z.add (BinIntDef.Z.of_nat 1)) (toN_int pred_tsize)) p .
+
+  Theorem fiat_pre_comp_table_gen_equiv : forall p,
+    to_list (fiat_pre_comp_table p) = fiat_pre_comp_table_gen 62%nat p.
+
+    intros. 
+    unfold fiat_pre_comp_table_gen, fiat_pre_comp_table, EC_fiat_P384_7.fiat_pre_comp_table.
+    removeCoerce.
+    removeCoerce.
+    rewrite toList_scanl_equiv.
+    Check ecFromTo_m_n_equiv.
+    replace (map (BinIntDef.Z.add (BinIntDef.Z.of_nat 1)) (toN_int 62))
+      with (to_list (ecFromTo (TCNum 1%nat) (TCNum 63%nat) Integer PLiteralInteger)).
+    reflexivity.
+    apply ecFromTo_m_n_equiv.
+  Qed.
+
+  
+  Definition fiat_double_add_body := 
+    fiat_double_add_body field_square field_mul field_sub field_add field_opp.
+  
+
+  Definition conditional_point_opp (t : bitvector 64) (p : point): point :=
+    Vector.cons (sawAt _ _ p 0%nat) (Vector.cons (fiat_field_cmovznz t (sawAt _ _ p 1%nat) (field_opp (sawAt _ _ p 1%nat))) (Vector.cons (sawAt _ _ p 2%nat) (Vector.nil _))).
+
+  Definition fiat_double_add_body_gen pred_wsize t p id :=
+    EC_fiat_P384_7.fiat_point_add field_square field_mul field_sub
+  field_add false
+  (fold_left
+     (fun
+        (x : CryptolPrimitivesForSAWCore.seq 3%nat
+               (CryptolPrimitivesForSAWCore.seq 6%nat
+                  (CryptolPrimitivesForSAWCore.seq 64%nat Bool)))
+        (_ : Integer) =>
+      fiat_point_double field_square field_mul field_sub field_add x)
+     (toN_int pred_wsize) p)
+  (conditional_point_opp
+     (point_id_to_limb
+        (bvAnd (shiftR 16 bool false id (S pred_wsize)) (bvNat 16%nat 1%nat)))
+     (fiat_select_point_ct_gen
+        (sign_extend_16_64
+           (bvSShr 15%nat
+              (bvAdd 16
+                 (bvXor 16%nat id
+                    (bvNeg 16
+                       (bvAnd (shiftR 16 bool false id (S pred_wsize))
+                          (bvNat 16%nat 1%nat))))
+                 (bvAnd (shiftR 16 bool false id (S pred_wsize))
+                    (bvNat 16%nat 1%nat))) 1%nat)) t)).
+
+  Theorem fiat_double_add_body_gen_equiv : forall t p id,
+    fiat_double_add_body t p id = fiat_double_add_body_gen 6 (to_list t) p id.
+
+    intros.
+    unfold fiat_double_add_body, EC_fiat_P384_7.fiat_double_add_body.
+    removeCoerce.
+    rewrite ecFoldl_foldl_equiv.
+    replace (to_list (ecFromTo 0%nat 6%nat Integer PLiteralInteger))
+      with (toN_int 6%nat).
+    repeat rewrite fiat_select_point_ct_gen_equiv.
+    reflexivity.
+
+    symmetry.
+    apply ecFromTo_0_n_equiv.
+
+  Qed.
+
+  Definition fiat_point_mul_gen wsize nw pred_tsize p s : point := 
+    EC_fiat_P384_7.conditional_subtract_if_even_ct field_square field_mul
+  field_sub field_add field_opp
+  (fold_left
+     (fiat_double_add_body_gen (pred wsize) (fiat_pre_comp_table_gen pred_tsize p))
+     (skipn 1 (rev (fiat_mul_scalar_rwnaf_gen wsize nw s)))
+     (fiat_select_point_ct_gen
+        (sign_extend_16_64
+           (bvSShr 15
+              (nth (S (S nw)) (fiat_mul_scalar_rwnaf_gen wsize nw s)
+                 (bvNat 16%nat 0%nat))
+              1%nat) )
+        (fiat_pre_comp_table_gen pred_tsize p))) s
+  (nth 0 (fiat_pre_comp_table_gen pred_tsize p)
+     (inhabitant (ecNumber 0%nat Integer PLiteralInteger))).
+
+  Theorem fiat_point_mul_gen_equiv : forall p s,
+    fiat_point_mul p s = fiat_point_mul_gen 7 52 62 p s.
+
+    intros.
+    unfold fiat_point_mul, EC_fiat_P384_7.fiat_point_mul.
+
+    rewrite ecFoldl_foldl_equiv.
+
+    Local Opaque fold_left.
+    simpl.
+    rewrite (fold_left_ext _
+      (fiat_double_add_body_gen 6%nat
+        (fiat_pre_comp_table_gen 62%nat p))
+    ).
+    rewrite toList_drop_equiv.
+    rewrite toList_reverse_equiv.
+    rewrite fiat_mul_scalar_rwnaf_equiv.
+
+    rewrite fiat_select_point_ct_gen_equiv.
+    rewrite fiat_pre_comp_table_gen_equiv.
+
+    unfold fiat_point_mul_gen.
+    rewrite sawAt_nth_equiv.
+    rewrite fiat_mul_scalar_rwnaf_equiv.
+
+    rewrite sawAt_nth_equiv.
+    rewrite fiat_pre_comp_table_gen_equiv.
+
+    reflexivity.
+
+    lia.
+    lia.
+
+    intros.
+    rewrite <- fiat_pre_comp_table_gen_equiv.
+    unfold fiat_pre_comp_table.
+  
+    rewrite <- fiat_double_add_body_gen_equiv.
+    reflexivity.
+
+  Qed.
+
+End PointMul.
+
+(*
+Definition fiat_mul_scalar_rwnaf_odd_loop_body_gen (wsize : nat)(s : CryptolPrimitivesForSAWCore.seq (CryptolPrimitivesForSAWCore.TCNum 384) SAWCoreScaffolding.Bool) (i : CryptolPrimitivesForSAWCore.seq (CryptolPrimitivesForSAWCore.TCNum 64) SAWCoreScaffolding.Bool)  :=
+    let var__0   := CryptolPrimitivesForSAWCore.TCNum 1 in
+    let var__1   := PZeroBit in let var__2   := PIntegralInteger in
+    let var__3   := PLiteralInteger in
+    let var__4   := CryptolPrimitivesForSAWCore.TCNum 7 in
+    let var__5   := CryptolPrimitivesForSAWCore.TCNum 384 in
+    let var__6   := CryptolPrimitivesForSAWCore.seq var__5 SAWCoreScaffolding.Bool in
+    let var__7   := CryptolPrimitivesForSAWCore.TCNum 32 in
+    let var__8   := CryptolPrimitivesForSAWCore.seq var__7 SAWCoreScaffolding.Bool in
+    let var__9   := CryptolPrimitivesForSAWCore.TCNum 16 in
+    let var__10   := CryptolPrimitivesForSAWCore.ecNumber var__4 SAWCoreScaffolding.Integer var__3 in
+    let var__11   := CryptolPrimitivesForSAWCore.ecNumber var__0 var__6 (CryptolPrimitivesForSAWCore.PLiteralSeqBool var__5) in
+    let var__12   := CryptolPrimitivesForSAWCore.PRingSeqBool var__5 in
+    let var__13   := CryptolPrimitivesForSAWCore.ecMinus var__6 var__12 (CryptolPrimitivesForSAWCore.ecAnd var__6 (CryptolPrimitivesForSAWCore.PLogicSeqBool var__5) s (CryptolPrimitivesForSAWCore.ecMinus var__6 var__12 (CryptolPrimitivesForSAWCore.ecShiftL var__5 SAWCoreScaffolding.Integer SAWCoreScaffolding.Bool var__2 var__1 var__11 (CryptolPrimitivesForSAWCore.ecPlus SAWCoreScaffolding.Integer PRingInteger var__10 (CryptolPrimitivesForSAWCore.ecNumber var__0 SAWCoreScaffolding.Integer var__3))) var__11)) (CryptolPrimitivesForSAWCore.ecShiftL var__5 SAWCoreScaffolding.Integer SAWCoreScaffolding.Bool var__2 var__1 var__11 var__10) in
+    let var__14   := CryptolPrimitivesForSAWCore.TCNum 368 in
+    let var__15   := CryptolPrimitivesForSAWCore.tcAdd var__14 var__9 in
+    pair 
+      (CryptolPrimitivesForSAWCore.ecDrop var__14 var__9 SAWCoreScaffolding.Bool 
+        var__13
+        
+      ) 
+      (shiftR _ _ false
+        (bvSub 
+          s 
+          (bvSub
+            (bvAnd
+              s 
+              (bvSub
+                (shiftL _ _ false
+                  var__11 
+                  (wsize + 1)
+                ) 
+                var__11
+              )
+            ) 
+            (CryptolPrimitivesForSAWCore.ecShiftL var__5 SAWCoreScaffolding.Integer SAWCoreScaffolding.Bool var__2 var__1 
+              var__11 
+              var__10
+            )
+          )
+        ) 
+        wsize
+      ).
+
+Theorem fiat_mul_scalar_rwnaf_odd_loop_body_0_gen_equiv : forall s i,
+  fiat_mul_scalar_rwnaf_odd_loop_body_gen_0 7 s i = fiat_mul_scalar_rwnaf_odd_loop_body_gen 7 s i.
+
+  intros.
+  reflexivity.
+
+Qed.
+
+Definition fiat_mul_scalar_rwnaf_odd_loop_body_gen (wsize : nat)
+(s : seq 384 bool) (i : seq 64 bool)  :=
+    let var__0   := CryptolPrimitivesForSAWCore.TCNum 1 in
+    let var__1   := PZeroBit in let var__2   := PIntegralInteger in
+    let var__3   := PLiteralInteger in
+    let var__4   := CryptolPrimitivesForSAWCore.TCNum 7 in
+    let var__5   := CryptolPrimitivesForSAWCore.TCNum 384 in
+    let var__6   := CryptolPrimitivesForSAWCore.seq var__5 SAWCoreScaffolding.Bool in
+    let var__7   := CryptolPrimitivesForSAWCore.TCNum 32 in
+    let var__8   := CryptolPrimitivesForSAWCore.seq var__7 SAWCoreScaffolding.Bool in
+    let var__9   := CryptolPrimitivesForSAWCore.TCNum 16 in
+    let var__10   := CryptolPrimitivesForSAWCore.seq var__9 SAWCoreScaffolding.Bool in
+    let var__11   := CryptolPrimitivesForSAWCore.ecNumber var__0 var__10 (CryptolPrimitivesForSAWCore.PLiteralSeqBool var__9) in
+    let var__12   := CryptolPrimitivesForSAWCore.ecNumber var__4 SAWCoreScaffolding.Integer var__3 in
+    let var__13   := CryptolPrimitivesForSAWCore.PRingSeqBool var__9 in
+    let var__14   := CryptolPrimitivesForSAWCore.TCNum 368 in
+    let var__15   := CryptolPrimitivesForSAWCore.tcAdd var__14 var__9 in
+    let var__16   := CryptolPrimitivesForSAWCore.ecMinus var__10 var__13 (CryptolPrimitivesForSAWCore.ecAnd var__10 (CryptolPrimitivesForSAWCore.PLogicSeqBool var__9) (CryptolPrimitivesForSAWCore.ecDrop var__14 var__9 SAWCoreScaffolding.Bool (SAWCoreScaffolding.coerce var__6 (CryptolPrimitivesForSAWCore.seq var__15 SAWCoreScaffolding.Bool) (CryptolPrimitivesForSAWCore.seq_cong1 var__5 var__15 SAWCoreScaffolding.Bool ltac:(solveUnsafeAssert)) s)) (CryptolPrimitivesForSAWCore.ecMinus var__10 var__13 (CryptolPrimitivesForSAWCore.ecShiftL var__9 SAWCoreScaffolding.Integer SAWCoreScaffolding.Bool var__2 var__1 var__11 (CryptolPrimitivesForSAWCore.ecPlus SAWCoreScaffolding.Integer PRingInteger var__12 (CryptolPrimitivesForSAWCore.ecNumber var__0 SAWCoreScaffolding.Integer var__3))) var__11)) (CryptolPrimitivesForSAWCore.ecShiftL var__9 SAWCoreScaffolding.Integer SAWCoreScaffolding.Bool var__2 var__1 var__11 var__12) in
+    
+let var__17   := CryptolPrimitivesForSAWCore.tcAdd var__9 var__14 in
+    pair var__16 
+      (shiftR _ _ false
+        (bvSub
+          s 
+          (sign_extend _ 368 
+            (CryptolPrimitivesForSAWCore.ecMinus _ var__13 
+              (bvAnd
+                (drop _ 368 _ s) 
+                (bvSub
+                  (shiftL _ _ false var__11 (wsize + 1)) 
+                  (bvNat _ 1)
+                )
+              ) 
+              (shiftL _ _ false (bvNat _ 1) wsize) 
+            )  
+          )
+        ) 
+        7
+      ).
+
+Theorem fiat_mul_scalar_rwnaf_odd_loop_body_gen_equiv : forall s i,
+  fiat_mul_scalar_rwnaf_odd_loop_body_gen 7 s i = fiat_mul_scalar_rwnaf_odd_loop_body s i.
+
+  intros.
+  reflexivity.
+
+Qed.
+  
+
+
+Print fiat_mul_scalar_rwnaf_odd_loop_body.
+
+(* Simplify fiat_mul_scalar_rwnaf_odd_loop_body. First remove all the SAW definitions. This is done in two steps to reduce
+the time required for reflexivity to complete. *)
+
+Definition fiat_mul_scalar_rwnaf_loop_body_gen_7 
+  (s : seq 384 Bool)(window : seq 16 Bool)(i : seq 64 Bool) : (seq 16 Bool * seq 16 Bool) :=
+
+    let var__0   := CryptolPrimitivesForSAWCore.TCNum 1 in
+    let var__1   := PZeroBit in 
+    let var__2   := PIntegralInteger in
+    let var__3   := PLiteralInteger in
+    let var__4   := TCNum 7 in
+    let var__5   := TCNum 64 in
+    let var__6   := seq var__5 Bool in
+    let var__7   := TCNum 32 in
+    let var__8   := seq var__7 Bool in
+    let var__9   := TCNum 48 in
+    let var__10   := PLiteralSeqBool var__7 in
+    let var__11   := TCNum 16 in
+    let var__12   := seq var__11 Bool in
+    let var__13   := tcAdd var__9 var__11 in
+    let var__14   := ecNumber var__0 var__12 (PLiteralSeqBool var__11) in
+    let var__15   := ecNumber var__4 Integer var__3 in
+    let var__16   := PRingSeqBool var__11 in
+    let var__17   := 
+      ecMinus var__12 var__16 (ecAnd var__12 (PLogicSeqBool var__11) window (ecMinus var__12 var__16 (ecShiftL var__11 Integer Bool var__2 var__1 var__14 (ecPlus Integer PRingInteger var__15 (ecNumber var__0 Integer var__3))) var__14)) (ecShiftL var__11 Integer Bool var__2 var__1 var__14 var__15) in
+    
+    
+    pair 
+      (bvSub 
+        (bvAnd window (bvSub (shiftL _ _ false var__14 (7 + 1)) var__14)) 
+        (shiftL _ _ false var__14 7)
+      )
+      (drop Bool 48 16 
+      (coerce (Vec 64 Bool) (Vec 64 Bool) 
+        (seq_cong1 var__5 var__13 Bool ltac:(solveUnsafeAssert)) 
+          (ecFoldl var__4 var__6 var__8 
+            (fun (a : var__6) (j : var__8) => 
+            bvAdd _ 
+              a 
+              (shiftL _ _ false 
+                (fiat_get_bit s 
+                  (bvAdd _ 
+                    (bvMul _ 
+                      (drop Bool 32 32 i) 
+                      (bvNat 32 7) 
+                    ) 
+                    (bvAdd _ (bvNat 32 7) j)
+                  )
+                ) 
+                (bvToNat _ j)
+              )
+            ) 
+          (bvAnd 
+            (shiftR _ _ false (bvSub (sign_extend_16_64 window) (sign_extend_16_64 var__17)) 7) 
+            (ecNumber (TCNum (Z.to_nat 33554431%Z)) var__6 (PLiteralSeqBool var__5))
+          ) 
+          (ecFromTo var__0 var__4 var__8 var__10)
+        ))).
+
+Theorem fiat_mul_scalar_rwnaf_loop_body_equiv_gen_7 : forall s w i,
+  fiat_mul_scalar_rwnaf_loop_body_gen_7 s w i = fiat_mul_scalar_rwnaf_loop_body s w i.
+
+  intros.
+  reflexivity.
+
+Qed.
+
+Definition bv16_1 := (Vector.append (Vector.const false 15) (Vector.cons true (Vector.nil _))).
+Definition wsize_mask wsize := (bvSub (shiftL _ _ false bv16_1 (wsize + 1)) bv16_1).
+
+Definition fiat_mul_scalar_rwnaf_loop_body_gen 
+  (wsize : nat)(s : seq 384 Bool)(window : seq 16 Bool)(i : seq 64 Bool) : (seq 16 Bool * seq 16 Bool) :=    
+    pair 
+      (bvSub 
+        (bvAnd window (bvSub (shiftL _ _ false bv16_1 (wsize + 1)) bv16_1)) 
+        (shiftL _ _ false bv16_1 wsize)
+      )
+      (drop Bool 48 16 
+        (foldl _ _ _
+          (fun (a : _) (j : _) => 
+            bvAdd _ 
+              a 
+              (shiftL _ _ false 
+                (fiat_get_bit s 
+                  (bvAdd _ 
+                    (bvMul _ 
+                      (drop Bool 32 32 i) 
+                      (bvNat 32 wsize) 
+                    ) 
+                    (bvAdd _ (bvNat 32 wsize) j)
+                  )
+                ) 
+                (bvToNat _ j)
+              )
+            ) 
+          (bvAnd 
+            (shiftR _ _ false 
+              (bvSub 
+                (sign_extend_16_64 window) 
+                (sign_extend_16_64 (bvSub  (bvAnd window (wsize_mask wsize)) (shiftL _ _ false bv16_1 wsize)))
+              ) 
+              wsize
+            ) 
+            (bvNat 64 (Z.to_nat 33554431%Z))
+          ) 
+          (gen (addNat 1 (subNat wsize 1)) _ (fun i : Nat => bvNat 32 (addNat i 1)))
+        )
+    ).
+
+
+Theorem fiat_mul_scalar_rwnaf_loop_body_gen_1_equiv : forall s w i,
+  fiat_mul_scalar_rwnaf_loop_body_gen_7 s w i = fiat_mul_scalar_rwnaf_loop_body_gen 7 s w i.
+  intros.
+  reflexivity.
+
+Qed.
+
+Definition bv64_bit b :=
+    (Vector.append (Vector.const false 63) (Vector.cons b (Vector.nil _))).
+
+(*
+Theorem foldl_get_bit_simpl : forall wsize i s1 s2 (ls : Vec 384 _) a,
+    (foldl _ _ _
+          (fun (a : _) (j : _) => 
+            bvAdd _ 
+              a 
+              (shiftL _ _ false 
+                (fiat_get_bit ls 
+                  (bvAdd _ 
+                    (bvMul _ 
+                      (drop Bool 32 32 i) 
+                      (bvNat 32 wsize) 
+                    ) 
+                    (bvAdd _ (bvNat 32 wsize) j)
+                  )
+                ) 
+                (bvToNat _ j)
+              )
+            ) 
+          a
+          (gen wsize _ (fun i : Nat => bvNat 32 (addNat i 1)))
+        ) = 
+        bvAdd _ a (fst (splitat ((bvToNat _ i) * wsize) (snd (splitat 1 ls)))).
+
+*)
+    
+
+Definition fiat_mul_scalar_rwnaf_gen (pred_numwindows : nat) (wsize : nat) (n : bitvector 384) :=
+
+  let xs := scanl (bitvector 64) (bitvector 16 * bitvector 16) pred_numwindows
+             (fun x => fiat_mul_scalar_rwnaf_loop_body_gen wsize n (snd x))
+             (intToBv 16 0,
+             append (intToBv 8 0)
+               (bvOr (bvAnd (drop Bool 376 8 n) (intToBv 8 255))
+                  (intToBv 8 1)))
+             (gen pred_numwindows (bitvector 64)
+                (fun i => intToBv 64 (Z.of_nat (addNat i 0)))) in
+
+  drop (bitvector 16) 1 (S pred_numwindows)
+    (append_comm
+       (SAWCorePrelude.map fst _ xs)
+       (cons 
+          (snd
+             (sawAt _ (bitvector 16 * bitvector 16)
+                (reverse xs)
+                0)) (nil (bitvector 16)))).
+
+Theorem scanl_ext : forall (A B : Type)(n : Nat)(f1 f2 : B -> A -> B) (ls : Vec n A) b,
+  (forall x y, (f1 x y) = (f2 x y)) ->
+  scanl _ _ n f1 b ls = scanl _ _ n f2 b ls.
+
+  induction ls; intuition; simpl in *.
+  f_equal.
+  rewrite H.
+  eauto.
+
+Qed.
+
+Theorem fiat_mul_scalar_rwnaf_equiv_gen : forall n,
+    fiat_mul_scalar_rwnaf_gen 54 7 n = fiat_mul_scalar_rwnaf n.
+Proof.
+  intro n.
+  Local Opaque scanl gen.
+  unfold fiat_mul_scalar_rwnaf_gen, fiat_mul_scalar_rwnaf.
+  rewrite (@scanl_ext _ _ _ 
+    (fun x : bitvector 16 * bitvector 16 =>
+            fiat_mul_scalar_rwnaf_loop_body_gen 7 n (snd x))
+    (fun __p0 : seq 16 Bool * seq 16 Bool =>
+                  fiat_mul_scalar_rwnaf_loop_body n (snd __p0))).
+  reflexivity.
+
+  intros.
+  rewrite <- fiat_mul_scalar_rwnaf_loop_body_gen_1_equiv.
+  eapply fiat_mul_scalar_rwnaf_loop_body_equiv_gen_7.
+Qed.
+
+
+Local Transparent scanl gen.
+
+Theorem drop1_cons_eq : forall (A : Type)(n : Nat)(ls : Vec n A) x,
+  (drop A 1 _ (cons x ls)) = ls.
+
+Admitted.
+
+Theorem sawAt0_cons_eq : forall (A : Type)(pf : Inhabited A)(n : Nat)(ls : Vec n A) x,
+  (@sawAt (S n) A pf (cons x ls) 0) = x.
+
+  intros.
+  unfold sawAt. trivial.
+
+Qed.
+
+
+Theorem sawAtS_cons_eq : forall (A : Type)(pf : Inhabited A)(n n' : Nat)(ls : Vec n A) x,
+  (@sawAt (S n) A pf (cons x ls) (S n')) = (@sawAt _ A pf ls n').
+
+  intros.
+  unfold sawAt. trivial.
+
+Qed.
+
+Theorem sawAt0_scanl_acc : forall (A C : Type)(pf : Inhabited A) f n ls acc,
+  (@sawAt (S n) A pf (scanl C A n f acc ls) 0) = acc.
+
+  intros.
+  unfold scanl.
+  destruct ls; simpl; rewrite sawAt0_cons_eq; trivial.
+
+Qed. 
+  
+
+Theorem drop_1_tl : forall (A : Type)(pf : Inhabited A)(n : Nat)(ls : Vec (S n) A),
+  (@drop _ pf 1 _ ls) = tl ls.
+
+Admitted.
+
+Theorem to_list_tl : forall (A : Type)(n : Nat)(ls : Vec (S n) A),
+  to_list (tl ls) = List.tl (to_list ls).
+Admitted.
+
+Theorem to_list_append_comm : forall (A : Type)(pf : Inhabited A)(n1 n2 : Nat)(ls1 : Vec n1 A)(ls2 : Vec n2 A),
+  @to_list A (addNat n2 n1) (@append_comm n1 n2 A pf ls1 ls2) = List.app (@to_list A n1 ls1) (@to_list A n2 ls2).
+Admitted.
+
+
+Theorem to_list_saw_map : forall (A B : Type)(pf : Inhabited A)(f : A -> B)(n : Nat)(ls : Vec n A),
+  to_list (SAWCorePrelude.map f n ls) = List.map f (to_list ls).
+Admitted.
+
+Theorem to_list_nil : forall (A : Type),
+  to_list (@nil A) = List.nil.
+Admitted.
+
+
+Theorem sawAt_eq_nth_list : forall (A : Type)(pf : Inhabited A)(n n' : Nat)(ls : Vec n A),
+  sawAt n A ls n' = List.nth n' (to_list ls) (inhabitant pf).
+
+Admitted.
+
+Theorem to_list_reverse : forall (A : Type)(pf : Inhabited A)(n : nat)(ls : Vec n A),
+  to_list (reverse ls) = List.rev (to_list ls).
+
+Admitted.
+
+Theorem last_eq_nth : forall (A : Type)(def : A)(ls : list A),
+  List.last ls def = List.nth (Datatypes.length ls - 1) ls def.
+
+  induction ls using rev_ind; intuition; simpl in *.
+  rewrite List.app_length; simpl.
+  rewrite app_nth2.
+  replace (Datatypes.length ls + 1 - 1 - Datatypes.length ls) with 0.
+  rewrite last_last.
+  trivial.
+  lia.
+  lia.
+
+Qed.
+
+
+Theorem nth_0_rev_eq_last : forall (A : Type)(def : A)(ls : list A),
+  List.nth 0 (List.rev ls) def = List.last ls def.
+
+  intros.
+  destruct ls. simpl; trivial.
+
+  rewrite rev_nth.
+  symmetry.
+  apply last_eq_nth.
+  simpl.
+  lia.
+
+Qed.
+
+Theorem scanl_cons : forall (A C : Type)(n : Nat)(ls : Vec n C) h f acc,
+  (scanl C A (S n) f acc (VectorDef.cons h ls)) =
+  VectorDef.cons acc (scanl C A n f (f acc h) ls) . 
+
+  intros. simpl in *. trivial.
+
+Qed.
+
+Fixpoint fold_list (A  C: Type)(f : A -> C -> (A * A))(ls : list C)(a : A) : list A :=
+  match ls with
+  | List.nil => a :: List.nil
+  | c :: ls' => let (x, a') := (f a c) in x :: (fold_list f ls' a')
+  end.
+
+Theorem fold_list_not_nil : forall (A C : Type)(f : A -> C -> (A * A))(ls : list C)(a : A),
+  fold_list f ls a <> List.nil.
+
+  induction ls; intuition; simpl in *.
+  discriminate.
+  remember (f a0 a) as z. destruct z.
+  discriminate.
+
+Qed.
+
+Theorem map_fst_scanl_pair : forall (A C : Type)(f : A -> C -> (A*A))(n : Nat) (ls : Vec n C) p,
+  List.map fst (to_list (scanl _ _ _ (fun x => f (snd x)) p ls)) = 
+  (fst p) :: (List.tl (List.map fst (to_list (scanl _ _ _ (fun x => f (snd x)) p ls)))).
+
+  induction ls; intuition.
+
+Qed.
+
+Theorem scanl_pair_eq_list :forall (A C : Type)(defA : A * A)(f : A -> C -> (A*A))(n : Nat) (ls : Vec n C) p,
+  List.tl
+  (List.map fst (to_list (scanl _ _ _ (fun x => f (snd x)) p ls)) ++
+   [snd (List.last (to_list (scanl _ _ _ (fun x => f (snd x)) p ls)) defA)]) =
+  fold_list f (to_list ls) (snd p).
+
+  induction ls.
+  intuition.
+
+  intros.
+  rewrite scanl_cons.
+  repeat rewrite to_list_cons.
+  simpl.
+  rewrite map_fst_scanl_pair.
+
+  specialize (IHls (f (snd p) h)).
+  destruct (to_list
+       (scanl C (A * A) n (fun x : A * A => f (snd x)) (f (snd p) h) ls)).
+  simpl in *.
+  exfalso.
+  eapply fold_list_not_nil.
+  symmetry. eauto.
+  remember (f (snd p) h) as z. destruct z.
+  simpl in *.
+  erewrite <- IHls.
+  reflexivity.
+
+Qed.
+
+Theorem scanl_pair_eq : 
+  forall (A C : Type)(pf : Inhabited A)(f : A -> C -> (A*A))(n : Nat) (ls : Vec n C) p,
+    to_list (drop _ 1 _ 
+      (append_comm 
+        (SAWCorePrelude.map fst _ (scanl _ _ _ (fun x => f (snd x)) p ls) ) 
+        (cons (snd (sawAt _ _ (reverse (scanl _ _ _ (fun x => f (snd x)) p ls) ) 0 )) (nil _))))
+    =   fold_list f (to_list ls) (snd p).
+
+  intros.
+  rewrite drop_1_tl.
+  rewrite to_list_tl.
+  match goal with
+  | [|- context[@to_list ?A ?n3 (@append_comm ?n1 ?n2 ?A ?pf ?ls1 ?ls2)]] =>
+    replace (@to_list A n3 (@append_comm n1 n2 A pf ls1 ls2)) 
+      with (List.app (@to_list A n1 ls1) (@to_list A n2 ls2)) ;
+    [idtac | symmetry ; eapply (@to_list_append_comm A pf n1 n2 ls1 ls2)]
+  end.
+  rewrite to_list_saw_map.
+  rewrite to_list_cons.
+  rewrite to_list_nil.
+  rewrite sawAt_eq_nth_list.
+  rewrite to_list_reverse.
+  rewrite nth_0_rev_eq_last.
+  eapply scanl_pair_eq_list.
+
+Qed.
+
+*)
